nola/iris/sinv.v
@@ -3,6 +3,7 @@
 From nola.iris Require Export ofe upd.
 From iris.algebra Require Import agree gmap_view.
 From iris.proofmode Require Import proofmode.
+Import OfeNotation.
 
 Implicit Type PROP : oFunctor.
 
