nola/iris/upd.v
@@ -296,44 +296,47 @@ Definition fupdw `{!BiFUpd PROP} (W : PROP) (E E' : coPset) (P : PROP) : PROP :=
 
 (** *** Notation *)
 
-Notation "|=[ W ] => P" := (bupdw W P)
-  (at level 99, P at level 200, format "'[  ' |=[ W ] =>  '/' P ']'")
-  : bi_scope.
-Notation "P =[ W ]=∗ Q" := (P -∗ |=[W]=> Q)%I
-  (at level 99, Q at level 200, format "'[' P  =[ W ]=∗  '/' '[' Q ']' ']'")
-  : bi_scope.
-Notation "P =[ W ]=∗ Q" := (P -∗ |=[W]=> Q) : stdpp_scope.
+Module UpdwNotation.
+  Notation "|=[ W ] => P" := (bupdw W P)
+    (at level 99, P at level 200, format "'[  ' |=[ W ] =>  '/' P ']'")
+    : bi_scope.
+  Notation "P =[ W ]=∗ Q" := (P -∗ |=[W]=> Q)%I
+    (at level 99, Q at level 200, format "'[' P  =[ W ]=∗  '/' '[' Q ']' ']'")
+    : bi_scope.
+  Notation "P =[ W ]=∗ Q" := (P -∗ |=[W]=> Q) : stdpp_scope.
 
-Notation "|=[ W ] { E , E' }=> P" := (fupdw W E E' P)
-  (at level 99, P at level 200,
-    format "'[  ' |=[ W ] '/' { E , E' }=>  '/' P ']'") : bi_scope.
-Notation "|=[ W ] { E }=> P" := (fupdw W E E P)
-  (at level 99, P at level 200, format "'[  ' |=[ W ] '/' { E }=>  '/' P ']'")
-  : bi_scope.
-Notation "P =[ W ] { E , E' }=∗ Q" := (P -∗ |=[W]{E,E'}=> Q)%I
-  (at level 99, Q at level 200,
-    format "'[' P  =[ W ] '/' { E , E' }=∗  '/' '[' Q ']' ']'") : bi_scope.
-Notation "P =[ W ] { E , E' }=∗ Q" := (P -∗ |=[W]{E,E'}=> Q) : stdpp_scope.
-Notation "P =[ W ] { E }=∗ Q" := (P -∗ |=[W]{E}=> Q)%I
-  (at level 99, Q at level 200,
-    format "'[' P  =[ W ] '/' { E }=∗  '/' '[' Q ']' ']'") : bi_scope.
-Notation "P =[ W ] { E }=∗ Q" := (P -∗ |=[W]{E}=> Q) : stdpp_scope.
+  Notation "|=[ W ] { E , E' }=> P" := (fupdw W E E' P)
+    (at level 99, P at level 200,
+      format "'[  ' |=[ W ] '/' { E , E' }=>  '/' P ']'") : bi_scope.
+  Notation "|=[ W ] { E }=> P" := (fupdw W E E P)
+    (at level 99, P at level 200, format "'[  ' |=[ W ] '/' { E }=>  '/' P ']'")
+    : bi_scope.
+  Notation "P =[ W ] { E , E' }=∗ Q" := (P -∗ |=[W]{E,E'}=> Q)%I
+    (at level 99, Q at level 200,
+      format "'[' P  =[ W ] '/' { E , E' }=∗  '/' '[' Q ']' ']'") : bi_scope.
+  Notation "P =[ W ] { E , E' }=∗ Q" := (P -∗ |=[W]{E,E'}=> Q) : stdpp_scope.
+  Notation "P =[ W ] { E }=∗ Q" := (P -∗ |=[W]{E}=> Q)%I
+    (at level 99, Q at level 200,
+      format "'[' P  =[ W ] '/' { E }=∗  '/' '[' Q ']' ']'") : bi_scope.
+  Notation "P =[ W ] { E }=∗ Q" := (P -∗ |=[W]{E}=> Q) : stdpp_scope.
 
-(** We move the position of [▷] to make the notation work *)
-Notation "|=[ W ] { E }▷[ E' ] => P" := (|=[W]{E,E'}=> ▷ |=[W]{E',E}=> P)%I
-  (at level 99, P at level 200,
-    format "'[  ' |=[ W ] '/' { E }▷[ E' ] =>  '/' P ']'") : bi_scope.
-Notation "|=[ W ] { E }▷=> P" := (|=[W]{E}=> ▷ |=[W]{E}=> P)%I
-  (at level 99, P at level 200,
-    format "'[  ' |=[ W ] '/' { E }▷=>  '/' P ']'") : bi_scope.
-Notation "|=[ W ] { E }▷[ E' ] =>^ n P" :=
-  (Nat.iter n (λ Q, |=[W]{E}▷[E'] => Q) P)%I
-  (at level 99, P at level 200, n at level 9,
-    format "'[  ' |=[ W ] '/' { E }▷[ E' ] =>^ n  '/' P ']'") : bi_scope.
-Notation "|=[ W ] { E }▷=>^ n P" :=
-  (Nat.iter n (λ Q, |=[W]{E}▷=> Q) P)%I
-  (at level 99, P at level 200, n at level 9,
-    format "'[  ' |=[ W ] '/' { E }▷=>^ n  '/' P ']'") : bi_scope.
+  (** We move the position of [▷] to make the notation work *)
+  Notation "|=[ W ] { E }▷[ E' ] => P" := (|=[W]{E,E'}=> ▷ |=[W]{E',E}=> P)%I
+    (at level 99, P at level 200,
+      format "'[  ' |=[ W ] '/' { E }▷[ E' ] =>  '/' P ']'") : bi_scope.
+  Notation "|=[ W ] { E }▷=> P" := (|=[W]{E}=> ▷ |=[W]{E}=> P)%I
+    (at level 99, P at level 200,
+      format "'[  ' |=[ W ] '/' { E }▷=>  '/' P ']'") : bi_scope.
+  Notation "|=[ W ] { E }▷[ E' ] =>^ n P" :=
+    (Nat.iter n (λ Q, |=[W]{E}▷[E'] => Q) P)%I
+    (at level 99, P at level 200, n at level 9,
+      format "'[  ' |=[ W ] '/' { E }▷[ E' ] =>^ n  '/' P ']'") : bi_scope.
+  Notation "|=[ W ] { E }▷=>^ n P" :=
+    (Nat.iter n (λ Q, |=[W]{E}▷=> Q) P)%I
+    (at level 99, P at level 200, n at level 9,
+      format "'[  ' |=[ W ] '/' { E }▷=>^ n  '/' P ']'") : bi_scope.
+End UpdwNotation.
+Import UpdwNotation.
 
 (** *** Lemmas *)
 Section lemmas.
