nola/prelude.v
@@ -3,8 +3,3 @@
   It gets imported and exported by all other files of [nola] *)
 
 From iris.prelude Require Export prelude.
-
-(** Nola notation scope *)
-Declare Scope nola_scope.
-Delimit Scope nola_scope with nola.
-Open Scope nola_scope.
