nola/util/intp.v
@@ -6,9 +6,8 @@ From nola Require Export prelude.
 Class Pintp (X A B : Type) := pintp : X → A → B.
 Hint Mode Pintp - ! - : typeclass_instances.
 Module PintpNotation.
-  Notation "⟦ ⟧( x )" := (pintp x) (format "⟦ ⟧( x )") : nola_scope.
-  Notation "⟦ ⟧( x )@{ A }" := (pintp (A:=A) x) (only parsing) : nola_scope.
-  Notation "⟦ a ⟧( x )" := (pintp x a) (format "⟦  '[' a  ']' ⟧( x )")
-    : nola_scope.
-  Notation "⟦ a ⟧( x )@{ A }" := (pintp (A:=A) x a) (only parsing) : nola_scope.
+  Notation "⟦ ⟧( x )" := (pintp x) (format "⟦ ⟧( x )").
+  Notation "⟦ ⟧( x )@{ A }" := (pintp (A:=A) x) (only parsing).
+  Notation "⟦ a ⟧( x )" := (pintp x a) (format "⟦  '[' a  ']' ⟧( x )").
+  Notation "⟦ a ⟧( x )@{ A }" := (pintp (A:=A) x a) (only parsing).
 End PintpNotation.
