nola/util/prod.v
@@ -11,14 +11,15 @@ Record prod' (A B : Type) : Type := pair' {
 Arguments pair' {_ _} _ _.
 Arguments fst' {_ _} _.
 Arguments snd' {_ _} _.
-Infix "*'" := prod' (at level 41, right associativity) : nola_scope.
-Notation "( a , .. , y , z )'" := (pair' a (.. (pair' y z) ..))
-  (format "( a ,  .. ,  y ,  z )'") : nola_scope.
-Notation "p .1'" := (fst' p) (at level 2, left associativity, format "p .1'")
-  : nola_scope.
-Notation "p .2'" := (snd' p) (at level 2, left associativity, format "p .2'")
-  : nola_scope.
-Notation "pl .*1'" := (fmap (M:=list) fst' pl)
-  (at level 2, left associativity, format "pl .*1'").
-Notation "pl .*2'" := (fmap (M:=list) snd' pl)
-  (at level 2, left associativity, format "pl .*2'").
+Infix "*'" := prod' (at level 41, right associativity).
+
+Module ProdNotation.
+  Notation "( a , .. , y , z )'" := (pair' a (.. (pair' y z) ..))
+    (format "( a ,  .. ,  y ,  z )'").
+  Notation "p .1'" := (fst' p) (at level 2, left associativity, format "p .1'").
+  Notation "p .2'" := (snd' p) (at level 2, left associativity, format "p .2'").
+  Notation "pl .*1'" := (fmap (M:=list) fst' pl)
+    (at level 2, left associativity, format "pl .*1'").
+  Notation "pl .*2'" := (fmap (M:=list) snd' pl)
+    (at level 2, left associativity, format "pl .*2'").
+End ProdNotation.
